rt spec+proof: update after merge
This mostly involves fixing mistakes made while resolving conflicts in
the merge commit. Some fixes are also needed in crefine to avoid name
clashes with bound variables that are now called xfdc.

Signed-off-by: Corey Lewis <corey.lewis@proofcraft.systems>

proof/invariant-abstract/BCorres2_AI.thy
@@ -26,8 +26,10 @@ locale BCorres2_AI =
 definition all_but_exst where
   "all_but_exst P \<equiv> (\<lambda>s. P (kheap s) (cdt s) (is_original_cap s)
                       (cur_thread s) (idle_thread s)
+                      (consumed_time s) (cur_time s)
+                      (cur_sc s) (reprogram_timer s)
                       (scheduler_action s) (domain_list s) (domain_index s)
-                      (cur_domain s) (domain_time s) (ready_queues s)
+                      (cur_domain s) (domain_time s) (ready_queues s) (release_queue s)
                       (machine_state s) (interrupt_irq_node s)
                       (interrupt_states s) (arch_state s))"
 
@@ -39,13 +41,14 @@ lemma ef_mk_ef: "empty_fail f \<Longrightarrow> mk_ef (f s) = f s"
   done
 
 lemma all_but_obvious:
-  "all_but_exst (\<lambda>kheap cdt is_original_cap cur_thread idle_thread
-       scheduler_action domain_list domain_index cur_domain domain_time
-       ready_queues machine_state interrupt_irq_node interrupt_states arch_state.
+  "all_but_exst (\<lambda>kheap cdt is_original_cap cur_thread idle_thread consumed_time cur_time cur_sc
+       reprogram_timer scheduler_action domain_list domain_index cur_domain domain_time
+       ready_queues release_queue  machine_state interrupt_irq_node interrupt_states arch_state.
        x = \<lparr>kheap = kheap, cdt = cdt, is_original_cap = is_original_cap, cur_thread = cur_thread,
-            idle_thread = idle_thread, scheduler_action = scheduler_action,
+            idle_thread = idle_thread, consumed_time = consumed_time, cur_time = cur_time,
+            cur_sc = cur_sc, reprogram_timer = reprogram_timer, scheduler_action = scheduler_action,
             domain_list = domain_list, domain_index = domain_index, cur_domain = cur_domain,
-            domain_time = domain_time, ready_queues = ready_queues,
+            domain_time = domain_time, ready_queues = ready_queues, release_queue = release_queue,
             machine_state = machine_state, interrupt_irq_node = interrupt_irq_node,
             interrupt_states = interrupt_states, arch_state = arch_state,
          exst = (exst x)\<rparr>) x"
