proof/invariant-abstract/ARM/ArchInterrupt_AI.thy
@@ -208,10 +208,6 @@ lemma empty_fail_maskInterrupt_ARCH[Interrupt_AI_assms]:
   "empty_fail (maskInterrupt f irq)"
   by (wp | simp add: maskInterrupt_def)+
 
-crunch timer_tick
-  for invs[wp]: invs
-  (wp: thread_set_invs_trivial[OF ball_tcb_cap_casesI])
-
 lemma (* handle_interrupt_invs *) [Interrupt_AI_assms]:
   "\<lbrace>invs\<rbrace> handle_interrupt irq \<lbrace>\<lambda>_. invs\<rbrace>"
   supply if_cong[cong]
