proof/refine/RISCV64/CSpace1_R.thy
@@ -1748,7 +1748,7 @@ lemma set_cap_not_quite_corres_prequel:
    apply (frule tcb_cases_related2)
    apply (clarsimp simp: set_cap_def2 split_def bind_def get_object_def
                          simpler_gets_def assert_def fail_def return_def
-                         set_object_def get_def put_def)
+                         set_object_def get_def put_def gets_the_def)
    apply (erule(2) pspace_relation_update_tcbs)
    apply (simp add: c)
   apply clarsimp
@@ -6750,7 +6750,7 @@ lemma cteSwap_corres:
     apply (erule (1) impE, assumption)
    apply (fastforce simp only: no_0_modify_map)
   apply (elim conjE TrueE, simp only:)
-  apply (drule (2) updateMDB_the_lot', fastforce simp only: no_0_modify_map)
+  apply (drule (2) updateMDB_the_lot', fastforce, simp only: no_0_modify_map)
   apply (drule in_getCTE, elim conjE, simp only:)
   apply (drule (2) updateMDB_the_lot', fastforce, simp only: no_0_modify_map)
   apply (elim conjE TrueE, simp only:)
