spec/abstract/KHeap_A.thy
@@ -541,6 +541,26 @@ definition reschedule_required :: "(unit, 'z::state_ext) s_monad" where
    od"
 
 definition
+  possible_switch_to :: "obj_ref \<Rightarrow> (unit, 'z::state_ext) s_monad" where
+  "possible_switch_to target \<equiv> do
+     sc_opt \<leftarrow> get_tcb_obj_ref tcb_sched_context target;
+     inq \<leftarrow> gets $ in_release_queue target;
+     when (sc_opt \<noteq> None \<and> \<not>inq) $ do
+       cur_dom \<leftarrow> gets cur_domain;
+       target_dom \<leftarrow> thread_get tcb_domain target;
+       action \<leftarrow> gets scheduler_action;
+       \<comment> \<open>not in @{text \<open>release queue & active_sc\<close>}\<close>
+       if target_dom \<noteq> cur_dom then
+         tcb_sched_action tcb_sched_enqueue target \<comment> \<open>not @{text \<open>in cur_domain\<close>}\<close>
+       else if action \<noteq> resume_cur_thread then do
+           reschedule_required;
+           tcb_sched_action tcb_sched_enqueue target
+         od
+       else set_scheduler_action $ switch_thread target
+     od
+   od"
+
+definition
   schedule_tcb :: "obj_ref \<Rightarrow> (unit, 'z::state_ext) s_monad"
 where
   "schedule_tcb tcb_ptr \<equiv> do
@@ -559,7 +579,6 @@ where
     schedulable \<leftarrow> gets (schedulable tcb_ptr);
     when (tcb_ptr = cur \<and> sched_act = resume_cur_thread \<and> \<not>schedulable) $ set_scheduler_action choose_new_thread
   od"
-
 
 (***)
 
@@ -622,121 +641,6 @@ text \<open>Tests whether an IRQ identifier is in use.\<close>
 definition
   is_irq_active :: "irq \<Rightarrow> (bool,'z::state_ext) s_monad" where
  "is_irq_active irq \<equiv> liftM (\<lambda>st. st \<noteq> IRQInactive) $ get_irq_state irq"
-
-
-definition
-  get_tcb_queue :: "domain \<Rightarrow> priority \<Rightarrow> (ready_queue, 'z::state_ext) s_monad" where
-  "get_tcb_queue d prio \<equiv> do
-     queues \<leftarrow> gets ready_queues;
-     return (queues d prio)
-   od"
-
-definition
-  set_tcb_queue :: "domain \<Rightarrow> priority \<Rightarrow> ready_queue \<Rightarrow> (unit, 'z::state_ext) s_monad" where
-  "set_tcb_queue d prio queue \<equiv>
-     modify (\<lambda>es. es\<lparr> ready_queues :=
-      (\<lambda>d' p. if d' = d \<and> p = prio then queue else ready_queues es d' p)\<rparr>)"
-
-definition
-  tcb_sched_action :: "(obj_ref \<Rightarrow> obj_ref list \<Rightarrow> obj_ref list) \<Rightarrow> obj_ref
-                        \<Rightarrow> (unit, 'z::state_ext) s_monad"
-where
-  "tcb_sched_action action thread \<equiv> do
-     d \<leftarrow> thread_get tcb_domain thread;
-     prio \<leftarrow> thread_get tcb_priority thread;
-     queue \<leftarrow> get_tcb_queue d prio;
-     set_tcb_queue d prio (action thread queue)
-   od"
-
-definition
-  tcb_sched_enqueue :: "obj_ref \<Rightarrow> obj_ref list \<Rightarrow> obj_ref list" where
-  "tcb_sched_enqueue thread queue \<equiv> if thread \<notin> set queue then thread # queue else queue"
-
-definition
-  tcb_sched_append :: "obj_ref \<Rightarrow> obj_ref list \<Rightarrow> obj_ref list" where
-  "tcb_sched_append thread queue \<equiv> if thread \<notin> set queue then queue @ [thread] else queue"
-
-definition
-  tcb_sched_dequeue :: "obj_ref \<Rightarrow> obj_ref list \<Rightarrow> obj_ref list" where
-  "tcb_sched_dequeue thread queue \<equiv> filter ((\<noteq>) thread) queue"
-
-definition
-  set_scheduler_action :: "scheduler_action \<Rightarrow> (unit, 'z::state_ext) s_monad" where
-  "set_scheduler_action action \<equiv>
-     modify (\<lambda>es. es\<lparr>scheduler_action := action\<rparr>)"
-
-definition
-  thread_set_priority :: "obj_ref \<Rightarrow> priority \<Rightarrow> (unit, 'z::state_ext) s_monad" where
-  "thread_set_priority tptr prio \<equiv> thread_set (\<lambda>tcb. tcb\<lparr>tcb_priority := prio\<rparr>) tptr"
-
-definition
-  thread_set_time_slice :: "obj_ref \<Rightarrow> nat \<Rightarrow> (unit, 'z::state_ext) s_monad" where
-  "thread_set_time_slice tptr time \<equiv> thread_set (\<lambda>tcb. tcb\<lparr>tcb_time_slice := time\<rparr>) tptr"
-
-definition
-  thread_set_domain :: "obj_ref \<Rightarrow> domain \<Rightarrow> (unit, 'z::state_ext) s_monad" where
-  "thread_set_domain tptr domain \<equiv> thread_set (\<lambda>tcb. tcb\<lparr>tcb_domain := domain\<rparr>) tptr"
-
-definition reschedule_required :: "(unit, 'z::state_ext) s_monad" where
-  "reschedule_required \<equiv> do
-     action \<leftarrow> gets scheduler_action;
-     case action of
-       switch_thread t \<Rightarrow> tcb_sched_action (tcb_sched_enqueue) t | _ \<Rightarrow> return ();
-     set_scheduler_action choose_new_thread
-   od"
-
-definition
-  possible_switch_to :: "obj_ref \<Rightarrow> (unit, 'z::state_ext) s_monad" where
-  "possible_switch_to target \<equiv> do
-     cur_dom \<leftarrow> gets cur_domain;
-     target_dom \<leftarrow> thread_get tcb_domain target;
-     action \<leftarrow> gets scheduler_action;
-
-     if (target_dom \<noteq> cur_dom) then
-       tcb_sched_action tcb_sched_enqueue target
-     else if (action \<noteq> resume_cur_thread) then do
-         reschedule_required;
-         tcb_sched_action tcb_sched_enqueue target
-       od
-     else set_scheduler_action $ switch_thread target
-   od"
-
-definition
-  set_thread_state_act :: "obj_ref \<Rightarrow> (unit, 'z::state_ext) s_monad"
-where
-  "set_thread_state_act tcb_ptr \<equiv> do
-    ts \<leftarrow> get_thread_state tcb_ptr;
-    cur \<leftarrow> gets cur_thread;
-    sched_act \<leftarrow> gets scheduler_action;
-    when (tcb_ptr = cur \<and> sched_act = resume_cur_thread \<and> \<not> runnable ts) $ set_scheduler_action choose_new_thread
-  od"
-
-(***)
-
-definition
-  set_thread_state :: "obj_ref \<Rightarrow> thread_state \<Rightarrow> (unit,'z::state_ext) s_monad"
-where
-  "set_thread_state ref ts \<equiv> do
-     tcb \<leftarrow> gets_the $ get_tcb ref;
-     set_object ref (TCB (tcb \<lparr> tcb_state := ts \<rparr>));
-     set_thread_state_act ref
-   od"
-
-definition
-  set_priority :: "obj_ref \<Rightarrow> priority \<Rightarrow> (unit,'z::state_ext) s_monad" where
-  "set_priority tptr prio \<equiv> do
-     tcb_sched_action tcb_sched_dequeue tptr;
-     thread_set_priority tptr prio;
-     ts \<leftarrow> get_thread_state tptr;
-     when (runnable ts) $ do
-       cur \<leftarrow> gets cur_thread;
-       if tptr = cur then reschedule_required else possible_switch_to tptr
-     od
-   od"
-
-definition
-  set_mcpriority :: "obj_ref \<Rightarrow> priority \<Rightarrow> (unit, 'z::state_ext) s_monad"  where
-  "set_mcpriority ref mcp \<equiv> thread_set (\<lambda>tcb. tcb\<lparr>tcb_mcpriority:=mcp\<rparr>) ref "
 
 
 section "User Context"
